ZipTest.lean
@@ -15,6 +15,7 @@ import ZipTest.NativeInflate
 import ZipTest.NativeGzip
 import ZipTest.NativeIntegration
 import ZipTest.NativeScale
+import ZipTest.NativeDeflate
 
 def main : IO Unit := do
   unless ← System.FilePath.pathExists "testdata" do
@@ -36,4 +37,5 @@ def main : IO Unit := do
   ZipTest.NativeGzip.tests
   ZipTest.NativeIntegration.tests
   ZipTest.NativeScale.tests
+  ZipTest.NativeDeflate.tests
   IO.println "\nAll tests passed!"
